app/models/ot/Operation.thy
@@ -26,7 +26,11 @@ cursor behind that elment
 \end{itemize}
 *}
 
-datatype 'char Action = Retain | Insert 'char | Delete 
+datatype 'char action = Retain | Insert 'char | Delete
+
+type_synonym 'char operation = "'char action list"
+
+type_synonym 'char document = "'char list"
 
 text {*
 An operation as an input length and an output length:
@@ -38,21 +42,44 @@ The output length is the length of the result of the application on a
 document on which the operation is defined.
 *}
 
-fun lengthBeforeOp :: "'char Action list \<Rightarrow> nat"
-where
-  "lengthBeforeOp [] = 0"
-| "lengthBeforeOp (Retain#next)    = Suc (lengthBeforeOp next)"
-| "lengthBeforeOp (Delete#next)    = Suc (lengthBeforeOp next)"
-| "lengthBeforeOp (Insert(_)#next) = lengthBeforeOp next"
+primrec lengthBeforeAction :: "'char action \<Rightarrow> nat" where
+  "lengthBeforeAction Retain     = 1"
+| "lengthBeforeAction Delete     = 1"
+| "lengthBeforeAction (Insert _) = 0"
 
-fun lengthAfterOp :: "'char Action list \<Rightarrow> nat"
-where
-  "lengthAfterOp [] = 0"
-| "lengthAfterOp (Retain#next)    = Suc (lengthAfterOp next)"
-| "lengthAfterOp (Delete#next)    = lengthAfterOp next"
-| "lengthAfterOp (Insert(_)#next) = Suc (lengthAfterOp next)"
+primrec lengthAfterAction :: "'char action \<Rightarrow> nat" where
+  "lengthAfterAction Retain     = 1"
+| "lengthAfterAction Delete     = 0"
+| "lengthAfterAction (Insert _) = 1"
 
-fun applyOp :: "'char Action list \<Rightarrow> 'char list \<Rightarrow> 'char list option"
+fun lengthBeforeOp :: "'char operation \<Rightarrow> nat" where
+  "lengthBeforeOp as = listsum (map lengthBeforeAction as)"
+
+fun lengthAfterOp :: "'char operation \<Rightarrow> nat"
+where
+  "lengthAfterOp as = listsum (map lengthAfterAction as)"
+
+lemma lengthBeforeCombines [simp]: "lengthBeforeOp a + lengthBeforeOp b = lengthBeforeOp (a@b)"
+  by (induct a, auto)
+
+lemma lengthAfterCombines [simp]: "lengthAfterOp a + lengthAfterOp b = lengthAfterOp (a@b)"
+  by (induct a, auto)
+
+inductive_set validOperations :: "('char operation \<times> 'char document \<times> 'char document) set" where
+  emptyDoc[intro!]: "([],[],[]) \<in> validOperations"
+| retain[intro!]:   "(a,d,d') \<in> validOperations \<Longrightarrow> (Retain#a,c#d,c#d')   \<in> validOperations"
+| delete[intro!]:   "(a,d,d') \<in> validOperations \<Longrightarrow> (Delete#a,c#d,d')     \<in> validOperations"
+| insert[intro!]:   "(a,d,d') \<in> validOperations \<Longrightarrow> ((Insert c)#a,d,c#d') \<in> validOperations"
+
+lemma lengthOfValidInput: "(a,d,d') \<in> validOperations \<Longrightarrow> lengthBeforeOp a = length d"
+  by (erule validOperations.induct, auto)
+
+lemma lengthOfValidOutput: "(a,d,d') \<in> validOperations \<Longrightarrow> lengthAfterOp a = length d'"
+  by (erule validOperations.induct, auto)
+
+(* TODO: Completeness of validOperations *)
+
+fun applyOp :: "'char operation \<Rightarrow> 'char document \<Rightarrow> 'char document option"
 where
   "applyOp ([])            ([])        = Some []"
 | "applyOp (Retain#next)   (head#tail) = Option.map (\<lambda>a. head#a) (applyOp next tail)"
@@ -66,50 +93,51 @@ text {* the application of an operation \texttt{a} to a document \texttt{d}
         yields a result iff the base length of the operation is equal to the
         length of the document *}
 
-lemma apply_complete: "(applyOp a d) = None \<longleftrightarrow> (lengthBeforeOp a) \<noteq> (length d)"
-  oops
+lemma validOperationApplyOp: "(a,d,d') \<in> validOperations \<Longrightarrow> applyOp a d = Some d'"
+  by (erule validOperations.induct, auto)
+
+(* TODO: applyOp = None => \<notin> validOperations ? *)
 
 subsection {* Composition of Operations *}
 
-fun addDeleteOp :: "'char Action list \<Rightarrow> 'char Action list"
+fun addDeleteOp :: "'char operation \<Rightarrow> 'char operation"
 where
   "addDeleteOp (Insert c#next) = (Insert c)#(addDeleteOp next)"
 | "addDeleteOp as = Delete#as"
 
-fun compose :: "'char Action list \<Rightarrow> 'char Action list \<Rightarrow> 'char Action list option"
+fun compose :: "'char operation \<Rightarrow> 'char operation \<Rightarrow> 'char operation option"
 where
-  "compose [] [] = Some []"
+  "compose [] []                        = Some []"
 | "compose (Delete#as)    (bs)          = Option.map (addDeleteOp) (compose as bs)"
 | "compose (as)           (Insert c#bs) = Option.map (\<lambda>a. Insert(c)#a) (compose as bs)"
 | "compose (Retain#as)    (Retain#bs)   = Option.map (\<lambda>a. Retain#a) (compose as bs)"
 | "compose (Retain#as)    (Delete#bs)   = Option.map (addDeleteOp) (compose as bs)"
 | "compose (Insert(c)#as) (Retain#bs)   = Option.map (\<lambda>a. Insert(c)#a) (compose as bs)"
 | "compose (Insert(_)#as) (Delete#bs)   = compose as bs"
-| "compose _ _ = None"
+| "compose _              _             = None"
 
-lemma compose_complete: "\<forall> a b. (lengthAfterOp a) = (lengthBeforeOp b) \<longleftrightarrow> isSome (compose a b)"  
-  oops
-
-lemma compose_inv: "\<forall> a b d. Option.bind (compose a b) (\<lambda>op'. applyOp op' d) 
-                           = Option.bind (applyOp a d) (\<lambda>d'. applyOp b d')"
-  oops
+lemma composeValidOperations: "(a,d,d') \<in> validOperations \<Longrightarrow> (b,d',d'') \<in> validOperations \<Longrightarrow> compose a b = Some ab"
 
 subsection {* Operation Transformation *}
 
-fun transform :: "'char Action list \<Rightarrow> 'char Action list \<Rightarrow> (('char Action list) \<times> ('char Action list)) option"
+fun transform :: "'char operation \<Rightarrow> 'char operation \<Rightarrow> ('char operation \<times> 'char operation) option"
 where
-  "transform [] [] = Some ([],[])"
-| "transform (Insert(c)#as) b        = Option.map (\<lambda>(at,bt). (Insert(c)#at,Retain#bt)) (transform as b)"
-| "transform a (Insert(c)#bs)        = Option.map (\<lambda>(at,bt). (Retain#at,Insert(c)#bt)) (transform a bs)"
-| "transform (Retain#as) (Retain#bs) = Option.map (\<lambda>(at,bt). (Retain#at,Retain#bt)) (transform as bs)"
-| "transform (Delete#as) (Delete#bs) = transform as bs"
-| "transform (Retain#as) (Delete#bs) = Option.map (\<lambda>(at,bt). (at,addDeleteOp(bt))) (transform as bs)"
-| "transform (Delete#as) (Retain#bs) = Option.map (\<lambda>(at,bt). (addDeleteOp(at),bt)) (transform as bs)"
-| "transform _ _ = None"
+  "transform []             []             = Some ([],[])"
+| "transform (Insert(c)#as) b              = Option.map (\<lambda>(at,bt). (Insert(c)#at,Retain#bt)) (transform as b)"
+| "transform a              (Insert(c)#bs) = Option.map (\<lambda>(at,bt). (Retain#at,Insert(c)#bt)) (transform a bs)"
+| "transform (Retain#as)    (Retain#bs)    = Option.map (\<lambda>(at,bt). (Retain#at,Retain#bt)) (transform as bs)"
+| "transform (Delete#as)    (Delete#bs)    = transform as bs"
+| "transform (Retain#as)    (Delete#bs)    = Option.map (\<lambda>(at,bt). (at,addDeleteOp(bt))) (transform as bs)"
+| "transform (Delete#as)    (Retain#bs)    = Option.map (\<lambda>(at,bt). (addDeleteOp(at),bt)) (transform as bs)"
+| "transform _              _              = None"
+
+text {* the transformation of two operations yields a result iff they have an equal input length *}
+lemma transform_complete: "(transform a b) = None \<longleftrightarrow> lengthBeforeOp a \<noteq> lengthBeforeOp b"
+  oops
 
 (* convergence property TP1 *)
-lemma transform_convergence: "\<forall> a b. Option.bind (transform a b) (\<lambda>(at,bt). compose a bt)
-                                   = Option.bind (transform a b) (\<lambda>(at,bt). compose b at)"
+lemma transform_convergence: "Option.bind (transform a b) (\<lambda>(at,bt). compose a bt)
+                            = Option.bind (transform a b) (\<lambda>(at,bt). compose b at)"
   oops
 
 export_code applyOp addDeleteOp compose transform in Scala
