app/assets/javascripts/config.coffee
@@ -1,2 +1,2 @@
 define ['app', 'config/routes'], (app, routes) ->
-  app.config routes  
+  app.config routes
