app/assets/javascripts/controllers/app.coffee
@@ -1,6 +1,7 @@
-define () -> ($scope, $location, App, Console) ->
+define () -> ($scope, $location, App, Console, Toasts) ->
   $scope.app = App
   $scope.console = Console
+  $scope.toasts = Toasts.toasts
   $scope.cm = 
   $scope.goBack = () ->
     window.history.back();
