app/assets/javascripts/controllers/login.coffee
@@ -1,23 +1,24 @@
-define ['routes'], (routes) -> ($scope,$location,App,Console) ->
-  $scope.username = 'martinring'
-  $scope.password = 'gNurz431'
-  $scope.login = () ->
+define ['routes'], (routes) -> ($scope,$location,App,Console,Toasts) ->
+  $scope.username = ''
+  $scope.password = ''
+  $scope.login = () ->    
     $scope.loginForm.error = null    
     App.wait = true
     Console.write "logging in as '#{$scope.username}'..."    
-    routes.controllers.Application.login().ajax      
+    routes.controllers.Application.login().ajax
       data: $('#loginForm').serialize()
       success: (data) ->
         App.loggedIn = true 
-        App.user = $scope.username       
+        App.user = $scope.username
         Console.write data, 'success'                
         $location.path "/#{$scope.username}/backstage"
+        Toasts.push('success',"You have been successfully logged in as #{$scope.username}!")
         App.wait = false        
         $scope.$apply()
       error: (data) -> switch data.status
         when 400          
           App.loggedIn = false
-          $scope.loginForm.error = data.responseText        
+          $scope.loginForm.error = data.responseText
           Console.write data.responseText, 'failure'
           App.wait = false
           $scope.$apply()
