app/assets/javascripts/controllers/signup.coffee
@@ -1,13 +1,32 @@
-define () -> ($scope,$location,App,Console) ->
+define ['routes'], (routes) -> ($scope,$location,App,Console) ->
+  $scope.username = ''
   $scope.email = ''
-  $scope.password = ''
-  $scope.login = () ->
-    Console.write "signing up as #{$scope.username}..."    
+  $scope.password = ''  
+  $scope.signup = () ->    
+    $scope.signupForm.error = null    
     App.wait = true
-    done = () ->
-      $location.path "/#{$scope.username}/backstage"
-      App.user = $scope.username
-      App.loggedIn = true
-      App.wait = false
-      $scope.$apply()
-    setTimeout(done,1000)
+    Console.write "signing up as '#{$scope.username}'..."
+    routes.controllers.Application.signup().ajax
+      data: $('#signupForm').serialize()
+      contentType: "application/json; charset=utf-8",
+      dataType: "json",
+      success: (data) ->
+        App.loggedIn = true
+        App.user = $scope.username
+        Console.write data, 'success'
+        $location.path "/#{$scope.username}/backstage"
+        App.wait = false
+        $scope.$apply()
+      error: (data) -> switch data.status
+        when 400
+          App.loggedIn = false
+          $scope.signupForm.error = data.responseText
+          Console.write data.responseText, 'failure'
+          App.wait = false
+          $scope.$apply()
+        when 404
+          App.loggedIn = false
+          $scope.signupForm.error = 'The server did not respond'
+          Console.write 'The server did not respont', 'failure'
+          App.wait = false
+          $scope.$apply()
