app/assets/javascripts/services.coffee
@@ -1,6 +1,7 @@
-define ['angular', 'services/projects', 'services/files', 'services/app', 'services/console'], (angular, projects, files, app, console) ->
+define ['angular', 'services/projects', 'services/files', 'services/app', 'services/console', 'services/toasts'], (angular, projects, files, app, console, toasts) ->
   module = angular.module 'clide.services', []  
   module.service 'Projects', projects
   module.service 'Files', files
   module.service 'App', app
   module.service 'Console', console  
+  module.service 'Toasts', toasts
