app/assets/javascripts/services/toasts.coffee
@@ -1,0 +1,20 @@
+define () -> ($rootScope) ->
+  toasts = []
+  push = (type, message) ->
+    toast = 
+      type: type
+      message: message    
+    toasts.push toast
+    toast.remove = () -> 
+      toasts.splice(toasts.indexOf(toast),1)
+      if (!$rootScope.$$phase)
+        $rootScope.$apply()
+    toast.reset = () ->      
+      toast.timeout = window.setTimeout(toast.remove, 5000) # TODO: move to settings
+    toast.reset()
+    if (!$rootScope.$$phase)
+      $rootScope.$apply()    
+  return (
+    toasts: toasts
+    push: push
+  )
